reconnect buffer backend with the double-fetch-freedom proof

src/3d/prelude/EverParse3d.InputBuffer.fst
@@ -10,54 +10,36 @@ module G = FStar.Ghost
 
 open LowParse.Low.Base
 
-inline_for_extraction
-noextract
-let base_t (len: U32.t)
-= (base: B.buffer LPL.byte { U32.v len <= B.length base })
-
-inline_for_extraction
-noextract
-noeq
-type input_buffer_perm (len: U32.t) = 
-{
-  p_base: Ghost.erased (base_t len);
-  p_perm: R.perm p_base;
-}
-
 let input_buffer_t len =
-  (p: (base_t len & input_buffer_perm len) { Ghost.reveal (snd p).p_base == fst p })
+  (base: B.buffer LPL.byte { U32.v len <= B.length base })
 
 let slice_of #len x =
-  { LPL.base = fst x; LPL.len = len }
+  { LPL.base = x; LPL.len = len }
 
-let perm_of x = (snd x).p_perm
-
-let drop sl from to =
-  match sl with
-  | (base, perm) ->
-    R.drop (perm.p_perm <: R.perm base) from to
+let drop #len base from to perm_of =
+    R.drop #byte #base perm_of from to
 
 (* TODO: remove the slice here *)
-let read_with_perm #k #t #p r #len sl pos =
-  match sl with
-  | (base, _) ->
-  [@inline_let] let sl' : LPL.slice triv triv = { LPL.base = base; LPL.len = len } in
+let read_with_perm #k #t #p r #len base pos n perm_of =
   let h0 = HST.get () in
+  LPL.valid_facts p h0 (slice_of base) pos;
+  LPL.parser_kind_prop_equiv k p;
+  [@inline_let] let sl' : LPL.slice triv triv = { LPL.base = base; LPL.len = pos `U32.add` n } in
+  LPL.parse_strong_prefix p (LPL.bytes_of_slice_from h0 (slice_of base) pos) (LPL.bytes_of_slice_from h0 sl' pos);
+  LPL.valid_facts p h0 sl' pos;
   let pos' = Ghost.hide (LPL.get_valid_pos p h0 sl' pos) in
   let res = r sl' pos in
   let h1 = HST.get () in
-  R.valid_perm_frame h0 (perm_of sl) B.loc_none h1;
-  R.preserved_split (perm_of sl) 0ul pos (B.len base) h0 h1;
-  R.preserved_split (perm_of sl) pos pos' (B.len base) h0 h1;
-  drop sl pos pos' ;
+  R.valid_perm_frame h0 perm_of B.loc_none h1;
+  R.preserved_split perm_of 0ul pos (B.len base) h0 h1;
+  R.preserved_split perm_of pos pos' (B.len base) h0 h1;
+  drop base pos pos' perm_of ;
   let h2 = HST.get () in
-  R.preserved_trans (perm_of sl) 0ul pos h0 h1 h2;
-  R.preserved_trans (perm_of sl) pos' (B.len base) h0 h1 h2;
+  R.preserved_trans perm_of 0ul pos h0 h1 h2;
+  R.preserved_trans perm_of pos' (B.len base) h0 h1 h2;
   res
 
 let puint8 = B.buffer LPL.byte
 
-let offset sl off =
-  match sl with
-  | (base, _) ->
+let offset base off perm_of =
   B.moffset triv base off
