src/3d/prelude/buffer/EverParse3d.Actions.All.fst
@@ -3,13 +3,15 @@ friend EverParse3d.Actions.Base
 friend EverParse3d.InputStream.All
 friend EverParse3d.InputStream.Buffer
 
-let ___PUINT8 = LowStar.Buffer.buffer FStar.UInt8.t
+module IB = EverParse3d.InputBuffer
+
+let ___PUINT8 = IB.puint8
 
 let action_field_ptr
       #nz #wk (#k:Prelude.parser_kind nz wk) (#t:Type) (#p:Prelude.parser k t) (u:unit)
    = fun ctxt input startPosition ->
        let open LowParse.Slice in
-       LowStar.Buffer.offset input.EverParse3d.InputStream.Buffer.Aux.buf (LowParse.Low.ErrorCode.uint64_to_uint32 startPosition)
+       IB.offset input.EverParse3d.InputStream.Buffer.Aux.buf (LowParse.Low.ErrorCode.uint64_to_uint32 startPosition) input.EverParse3d.InputStream.Buffer.Aux.perm_of
 
 let action_field_pos_32
       #nz #wk (#k:Prelude.parser_kind nz wk) (#t:Type) (#p:Prelude.parser k t) (u:unit)
